revert "join" for nat/int in FStar.Integer

ulib/FStar.Integers.fst
@@ -1,20 +1,6 @@
 module FStar.Integers
 
 #set-options "--initial_ifuel 1 --max_ifuel 1 --initial_fuel 0 --max_fuel 0"
-irreducible
-private
-let mark_for_norm = ()
-
-irreducible
-private
-let attr_join = ()
-
-unfold
-let norm_join (#a:Type) (x:a) =
-   if true then norm [iota; primops; delta_attr attr_join] x else x
-
-unfold
-let norm (#a:Type) (x:a) = norm [iota; primops; delta_attr mark_for_norm] x
 
 type signedness =
   | Signed
@@ -32,23 +18,6 @@ type width =
 
 let fixed_width = w:width{w <> Winfinite}
 
-[@mark_for_norm attr_join]
-let join (s1, w1) (s2, w2) =
-  match w1, w2 with
-  | Winfinite, Winfinite ->
-    //Any operation on infinite width types
-    //uses the full range of mathematical integers
-    //This is to support the existing behavior from Prims
-    //of the basic arithmetic operations being defined on Prims.int
-    Some (Signed, Winfinite)
-
-  | _ ->
-    //No other heterogeneous combinations are supported
-    if (s1, w1) = (s2, w2)
-    then Some (s1, w1)
-    else None
-
-[@mark_for_norm]
 let nat_of_width = function
   | W8   -> Some 8
   | W16  -> Some 16
@@ -59,13 +28,10 @@ let nat_of_width = function
   | W128 -> Some 128
   | Winfinite -> None
 
-[@mark_for_norm]
 let nat_of_fixed_width (w:fixed_width) =
   match nat_of_width w with
   | Some v -> v
 
-[@mark_for_norm]
-inline_for_extraction
 let int_t (s:signedness) (w:width) : Tot Type0 =
   match s, w with
   | Unsigned, Winfinite -> nat
@@ -85,37 +51,39 @@ let int_t (s:signedness) (w:width) : Tot Type0 =
   | Signed, W64 -> FStar.Int64.t
   | Signed, W128 -> FStar.Int128.t
 
-[@mark_for_norm attr_join]
-inline_for_extraction
-let join_types #s1 #w1 (x:int_t s1 w1)
-               #s2 #w2 (y:int_t s2 w2{Some? (join (s1, w1) (s2, w2))}) : Type0 =
-  let Some (s, w) = join (s1, w1) (s2, w2) in
-  int_t s w
+abstract
+let nat_size (x:int) : Type =
+  x >= 0
+let reveal_nat_size x
+  : Lemma (nat_size x <==> x >= 0)
+          [SMTPat (nat_size x)]
+  = ()
 
-[@mark_for_norm]
-let within_bounds' (s:signedness) (w:width) (x:int) =
+abstract
+let uint_size (x:int) (n:nat) : Type =
+    FStar.UInt.size x n
+let reveal_uint_size x n
+  : Lemma (uint_size x n <==> FStar.UInt.size x n)
+          [SMTPat (uint_size x n)]
+  = ()
+
+abstract
+let int_size (x:int) (n:pos) : Type =
+    FStar.Int.size x n
+let reveal_int_size x n
+  : Lemma (int_size x n <==> FStar.Int.size x n)
+          [SMTPat (int_size x n)]
+  = ()
+
+let within_bounds (s:signedness) (w:width) (x:int) =
   match s, nat_of_width w with
   | Signed,   None   -> True
-  | Unsigned, None   -> b2t (x >= 0)
-  | Signed  , Some n -> FStar.Int.size x n
-  | Unsigned, Some n -> FStar.UInt.size x n
+  | Unsigned, None   -> nat_size x
+  | Signed  , Some n -> int_size x n
+  | Unsigned, Some n -> uint_size x n
 
-[@mark_for_norm]
-unfold
-let within_bounds s w x = norm (within_bounds' s w x)
-
-[@mark_for_norm attr_join]
-unfold
-let join_within_bounds #s1 #w1 (_:int_t s1 w1)
-                       #s2 #w2 (_:int_t s2 w2)
-                       (x:Prims.int) =
-  norm (match join (s1, w1) (s2, w2) with
-        | None -> False
-        | Some (s, w) -> within_bounds' s w x)
-
-[@mark_for_norm]
 let v (#s:signedness) (#w:width) (x:int_t s w)
-  : Tot (y:int_t Signed Winfinite{within_bounds s w y})
+  : Tot (y:int_t Signed Winfinite{normalize (within_bounds s w y)})
   = match s with
     | Unsigned ->
       (match w with
@@ -138,10 +106,9 @@ let v (#s:signedness) (#w:width) (x:int_t s w)
        | W64 -> FStar.Int64.v x
        | W128 -> FStar.Int128.v x)
 
-[@mark_for_norm]
 let u   (#s:signedness) (#w:width)
-        (x:int_t Signed Winfinite{within_bounds s w x})
-  : Tot (y:int_t s w{norm (v x == v y)})
+        (x:int_t Signed Winfinite{normalize (within_bounds s w x)})
+  : Tot (y:int_t s w{normalize (v x == v y)})
   = match s with
     | Unsigned ->
       (match w with
@@ -164,31 +131,18 @@ let u   (#s:signedness) (#w:width)
        | W64 -> FStar.Int64.int_to_t x
        | W128 -> FStar.Int128.int_to_t x)
 
-[@mark_for_norm attr_join]
-let v_join #s1 #w1 (_x:int_t s1 w1)
-           #s2 #w2 (_y:int_t s2 w2{Some? (join (s1, w1) (s2, w2))})
-           (z:join_types _x _y)
-  : Tot (w:int_t Signed Winfinite{join_within_bounds _x _y w})
-  = let Some (s, w) = join (s1, w1) (s2, w2) in
-    v #s #w z
-
-abstract
-let cast (#s:signedness) (#s':signedness)
+abstract let cast (#s:signedness) (#s':signedness)
          (#w:width)      (#w':width)
-         (from:int_t s w{within_bounds s' w' (v from)})
-   : Tot (to:int_t s' w'{norm (v from == v to)})
+         (from:int_t s w{normalize (within_bounds s' w' (v from))})
+   : Tot (to:int_t s' w'{normalize (v from == v to)})
    = u (v from)
 
-[@mark_for_norm]
 unfold
-private
-let addition (#s1:signedness) (#w1:width)
-             (#s2:signedness) (#w2:width)
-             (x:int_t s1 w1)
-             (y:int_t s2 w2{join_within_bounds x y (v x + v y)})
-  : Tot   (z:join_types x y) //{norm (v z == v x + v y)})
-  = let Some (s, w) = join (s1, w1) (s2, w2) in
-    match s, w with
+let ( + ) (#s:signedness) (#w:width)
+          (x:int_t s w)
+          (y:int_t s w{normalize (within_bounds s w (v x + v y))})
+  : Tot   (z:int_t s w{normalize (v z = v x + v y)})
+  = match s, w with
     | _, Winfinite -> x + y
     | Unsigned, W8   -> FStar.UInt8.(x +^ y)
     | Unsigned, W16  -> FStar.UInt16.(x +^ y)
@@ -205,278 +159,187 @@ let addition (#s1:signedness) (#w1:width)
     | Signed, W64  -> FStar.Int64.(x +^ y)
     | Signed, W128 -> FStar.Int128.(x +^ y)
 
-[@mark_for_norm]
 unfold
-let ( + ) (#s1:signedness) (#w1:width)
-             (#s2:signedness) (#w2:width)
-             (x:int_t s1 w1)
-             (y:int_t s2 w2) //{join_within_bounds x y (v x + v y)})
-  : Tot   (z:norm_join (join_types x y)) //{norm (v z == v x + v y)})
-  = x `addition` y
+let ( +? ) (#w:width)
+           (x:int_t Unsigned w)
+           (y:int_t Unsigned w)
+  : Tot    (z:int_t Unsigned w{normalize (within_bounds Unsigned w (v x + v y) ==> v z = v x + v y)})
+  = match w with
+    | Winfinite -> x + y
+    | W8 -> FStar.UInt8.(x +?^ y)
+    | W16 -> FStar.UInt16.(x +?^ y)
+    | W31 -> FStar.UInt31.(x +?^ y)
+    | W32 -> FStar.UInt32.(x +?^ y)
+    | W63 -> FStar.UInt63.(x +?^ y)
+    | W64 -> FStar.UInt64.(x +?^ y)
+    | W128 -> FStar.UInt128.(x +?^ y)
 
-#set-options "--debug Rel --debug_level RelDelta"
-let test (x:int_t Unsigned W32) (y:int_t Unsigned W32) (z:norm_join (join_types x y)) =
-  assume False;
-  x + z
+let modulo (s:signedness) (x:int) (y:pos{s=Signed ==> y%2=0}) =
+  match s with
+  | Unsigned ->  x % y
+  | _ -> FStar.Int.(x @% y)
 
+unfold
+let ( +% ) (#w:fixed_width)
+           (x:int_t Unsigned w)
+           (y:int_t Unsigned w)
+  : Tot    (z:int_t Unsigned w{v z == modulo Unsigned (v x + v y) (pow2 (nat_of_fixed_width w))})
+  = match w with
+    | W8 -> FStar.UInt8.(x +%^ y)
+    | W16 -> FStar.UInt16.(x +%^ y)
+    | W31 -> FStar.UInt31.(x +%^ y)
+    | W32 -> FStar.UInt32.(x +%^ y)
+    | W63 -> FStar.UInt63.(x +%^ y)
+    | W64 -> FStar.UInt64.(x +%^ y)
+    | W128 -> FStar.UInt128.(x +%^ y)
 
-//   x + y + y
+unfold
+let op_Subtraction (#s:signedness) (#w:width)
+                   (x:int_t s w)
+                   (y:int_t s w{within_bounds s w (v x - v y)})
+    : Tot          (z:int_t s w{v z = v x - v y})
+  = match s, w with
+    | _, Winfinite -> x - y
+    | Unsigned, W8 -> FStar.UInt8.(x -^ y)
+    | Unsigned, W16 -> FStar.UInt16.(x -^ y)
+    | Unsigned, W31 -> FStar.UInt31.(x -^ y)
+    | Unsigned, W32 -> FStar.UInt32.(x -^ y)
+    | Unsigned, W63 -> FStar.UInt63.(x -^ y)
+    | Unsigned, W64 -> FStar.UInt64.(x -^ y)
+    | Unsigned, W128 -> FStar.UInt128.(x -^ y)
+    | Signed, W8 -> FStar.Int8.(x -^ y)
+    | Signed, W16 -> FStar.Int16.(x -^ y)
+    | Signed, W31 -> FStar.Int31.(x -^ y)
+    | Signed, W32 -> FStar.Int32.(x -^ y)
+    | Signed, W63 -> FStar.Int63.(x -^ y)
+    | Signed, W64 -> FStar.Int64.(x -^ y)
+    | Signed, W128 -> FStar.Int128.(x -^ y)
 
-// [@mark_for_norm]
-// unfold
-// let ( +? ) (#w:width)
-//            (x:int_t Unsigned w)
-//            (y:int_t Unsigned w)
-//   : Tot    (z:int_t Unsigned w) //{within_bounds Unsigned w (v x + v y) ==> norm (v z == v x + v y)})
-//   = match w with
-//     | Winfinite -> x + y
-//     | W8 -> FStar.UInt8.(x +?^ y)
-//     | W16 -> FStar.UInt16.(x +?^ y)
-//     | W31 -> FStar.UInt31.(x +?^ y)
-//     | W32 -> FStar.UInt32.(x +?^ y)
-//     | W63 -> FStar.UInt63.(x +?^ y)
-//     | W64 -> FStar.UInt64.(x +?^ y)
-//     | W128 -> FStar.UInt128.(x +?^ y)
+unfold
+let op_Subtraction_Question
+        (#w:width)
+        (x:int_t Unsigned w)
+        (y:int_t Unsigned w)
+  : Tot (z:int_t Unsigned w{within_bounds Unsigned w (v x - v y) ==> v z = v x - v y})
+  = match w with
+    | Winfinite -> if v x - v y >= 0 then x - y else 0
+    | W8 -> FStar.UInt8.(x -?^ y)
+    | W16 -> FStar.UInt16.(x -?^ y)
+    | W31 -> FStar.UInt31.(x -?^ y)
+    | W32 -> FStar.UInt32.(x -?^ y)
+    | W63 -> FStar.UInt63.(x -?^ y)
+    | W64 -> FStar.UInt64.(x -?^ y)
+    | W128 -> FStar.UInt128.(x -?^ y)
 
-// [@mark_for_norm]
-// let modulo (s:signedness) (x:int) (y:pos{s=Signed ==> y%2=0}) =
-//   match s with
-//   | Unsigned ->  x % y
-//   | _ -> FStar.Int.(x @% y)
+unfold
+let op_Subtraction_Percent
+         (#w:fixed_width)
+         (x:int_t Unsigned w)
+         (y:int_t Unsigned w)
+  : Tot  (z:int_t Unsigned w{v z = modulo Unsigned (v x - v y) (pow2 (nat_of_fixed_width w))})
+  = match w with
+    | W8 -> FStar.UInt8.(x -%^ y)
+    | W16 -> FStar.UInt16.(x -%^ y)
+    | W31 -> FStar.UInt31.(x -%^ y)
+    | W32 -> FStar.UInt32.(x -%^ y)
+    | W63 -> FStar.UInt63.(x -%^ y)
+    | W64 -> FStar.UInt64.(x -%^ y)
+    | W128 -> FStar.UInt128.(x -%^ y)
 
-// [@mark_for_norm]
-// unfold
-// let ( +% ) (#w:fixed_width)
-//            (x:int_t Unsigned w)
-//            (y:int_t Unsigned w)
-//   : Tot    (z:int_t Unsigned w) //{norm (v z == modulo Unsigned (v x + v y) (pow2 (nat_of_fixed_width w)))})
-//   = match w with
-//     | W8 -> FStar.UInt8.(x +%^ y)
-//     | W16 -> FStar.UInt16.(x +%^ y)
-//     | W31 -> FStar.UInt31.(x +%^ y)
-//     | W32 -> FStar.UInt32.(x +%^ y)
-//     | W63 -> FStar.UInt63.(x +%^ y)
-//     | W64 -> FStar.UInt64.(x +%^ y)
-//     | W128 -> FStar.UInt128.(x +%^ y)
+open FStar.Mul
 
-// [@mark_for_norm]
-// unfold
-// private
-// let subtraction (#s1:signedness) (#w1:width) (#s2:signedness) (#w2:width)
-//                    (x:int_t s1 w1) (y:int_t s2 w2{join_within_bounds x y (v x - v y)})
-//     : Tot          (z:join_types x y)
-//   = let Some (s, w) = join (s1, w1) (s2, w2) in
-//     match s, w with
-//     | _, Winfinite -> x - y
-//     | Unsigned, W8 -> FStar.UInt8.(x -^ y)
-//     | Unsigned, W16 -> FStar.UInt16.(x -^ y)
-//     | Unsigned, W31 -> FStar.UInt31.(x -^ y)
-//     | Unsigned, W32 -> FStar.UInt32.(x -^ y)
-//     | Unsigned, W63 -> FStar.UInt63.(x -^ y)
-//     | Unsigned, W64 -> FStar.UInt64.(x -^ y)
-//     | Unsigned, W128 -> FStar.UInt128.(x -^ y)
-//     | Signed, W8 -> FStar.Int8.(x -^ y)
-//     | Signed, W16 -> FStar.Int16.(x -^ y)
-//     | Signed, W31 -> FStar.Int31.(x -^ y)
-//     | Signed, W32 -> FStar.Int32.(x -^ y)
-//     | Signed, W63 -> FStar.Int63.(x -^ y)
-//     | Signed, W64 -> FStar.Int64.(x -^ y)
-//     | Signed, W128 -> FStar.Int128.(x -^ y)
+unfold
+let ( * ) (#s:signedness) (#w:width{w <> W128})
+          (x:int_t s w)
+          (y:int_t s w{within_bounds s w (v x * v y)})
+  : Tot   (z:int_t s w{v z = v x * v y})
+  = match s, w with
+    | _, Winfinite -> x * y
+    | Unsigned, W8 -> FStar.UInt8.(x *^ y)
+    | Unsigned, W16 -> FStar.UInt16.(x *^ y)
+    | Unsigned, W31 -> FStar.UInt31.(x *^ y)
+    | Unsigned, W32 -> FStar.UInt32.(x *^ y)
+    | Unsigned, W63 -> FStar.UInt63.(x *^ y)
+    | Unsigned, W64 -> FStar.UInt64.(x *^ y)
+    | Signed, W8 -> FStar.Int8.(x *^ y)
+    | Signed, W16 -> FStar.Int16.(x *^ y)
+    | Signed, W31 -> FStar.Int31.(x *^ y)
+    | Signed, W32 -> FStar.Int32.(x *^ y)
+    | Signed, W63 -> FStar.Int63.(x *^ y)
+    | Signed, W64 -> FStar.Int64.(x *^ y)
+    | Signed, W128 -> FStar.Int128.(x *^ y)
 
-// [@mark_for_norm]
-// unfold
-// private
-// let op_Subtraction (#s1:signedness) (#w1:width) (#s2:signedness) (#w2:width)
-//                    (x:int_t s1 w1) (y:int_t s2 w2{join_within_bounds x y (v x - v y)})
-//     : Tot (z:norm (norm_join (join_types x y)))
-//     = x `subtraction` y
+unfold
+let ( *? ) (#w:width{w <> W128})
+           (x:int_t Unsigned w)
+           (y:int_t Unsigned w)
+  : Tot    (z:int_t Unsigned w{within_bounds Unsigned w (v x * v y) ==> v z = v x * v y})
+  = match w with
+    | Winfinite -> x * y
+    | W8 -> FStar.UInt8.(x *?^ y)
+    | W16 -> FStar.UInt16.(x *?^ y)
+    | W31 -> FStar.UInt31.(x *?^ y)
+    | W32 -> FStar.UInt32.(x *?^ y)
+    | W63 -> FStar.UInt63.(x *?^ y)
+    | W64 -> FStar.UInt64.(x *?^ y)
 
-// [@mark_for_norm]
-// unfold
-// let op_Subtraction_Question
-//         (#w:width)
-//         (x:int_t Unsigned w)
-//         (y:int_t Unsigned w)
-//   : Tot (z:int_t Unsigned w) //{within_bounds Unsigned w (v x - v y) ==> norm (v z == v x - v y)})
-//   = match w with
-//     | Winfinite -> if v x - v y >= 0 then x - y else 0
-//     | W8 -> FStar.UInt8.(x -?^ y)
-//     | W16 -> FStar.UInt16.(x -?^ y)
-//     | W31 -> FStar.UInt31.(x -?^ y)
-//     | W32 -> FStar.UInt32.(x -?^ y)
-//     | W63 -> FStar.UInt63.(x -?^ y)
-//     | W64 -> FStar.UInt64.(x -?^ y)
-//     | W128 -> FStar.UInt128.(x -?^ y)
+unfold
+let ( *% ) (#w:fixed_width{w <> W128})
+           (x:int_t Unsigned w)
+           (y:int_t Unsigned w)
+  : Tot    (z:int_t Unsigned w{v z = modulo Unsigned (v x * v y) (pow2 (nat_of_fixed_width w))})
+  = match w with
+    | W8 -> FStar.UInt8.(x *%^ y)
+    | W16 -> FStar.UInt16.(x *%^ y)
+    | W31 -> FStar.UInt31.(x *%^ y)
+    | W32 -> FStar.UInt32.(x *%^ y)
+    | W63 -> FStar.UInt63.(x *%^ y)
+    | W64 -> FStar.UInt64.(x *%^ y)
 
-// [@mark_for_norm]
-// unfold
-// let op_Subtraction_Percent
-//          (#w:fixed_width)
-//          (x:int_t Unsigned w)
-//          (y:int_t Unsigned w)
-//   : Tot  (z:int_t Unsigned w) //{norm (v z == modulo Unsigned (v x - v y) (pow2 (nat_of_fixed_width w)))})
-//   = match w with
-//     | W8 -> FStar.UInt8.(x -%^ y)
-//     | W16 -> FStar.UInt16.(x -%^ y)
-//     | W31 -> FStar.UInt31.(x -%^ y)
-//     | W32 -> FStar.UInt32.(x -%^ y)
-//     | W63 -> FStar.UInt63.(x -%^ y)
-//     | W64 -> FStar.UInt64.(x -%^ y)
-//     | W128 -> FStar.UInt128.(x -%^ y)
+unfold let nat        = int_t Unsigned Winfinite
+unfold let uint_8   = int_t Unsigned W8
+unfold let uint_16  = int_t Unsigned W16
+unfold let uint_31  = int_t Unsigned W31
+unfold let uint_32  = int_t Unsigned W32
+unfold let uint_63  = int_t Unsigned W63
+unfold let uint_64  = int_t Unsigned W64
 
-// open FStar.Mul
+unfold let int       = int_t Signed Winfinite
+unfold let int_8   = int_t Signed W8
+unfold let int_16  = int_t Signed W16
+unfold let int_31  = int_t Signed W31
+unfold let int_32  = int_t Signed W32
+unfold let int_63  = int_t Signed W63
+unfold let int_64  = int_t Signed W64
+unfold let int_128 = int_t Signed W128
 
-// [@mark_for_norm]
-// unfold
-// private
-// let multiplication (#s1:signedness) (#w1:width{w1 <> W128}) (#s2:signedness) (#w2:width{w2 <> W128})
-//                    (x:int_t s1 w1) (y:int_t s2 w2{join_within_bounds x y (v x * v y)})
-//   : Tot   (z:join_types x y)
-//   = let Some (s, w) = join (s1, w1) (s2, w2) in
-//     match s, w with
-//     | _, Winfinite -> x * y
-//     | Unsigned, W8 -> FStar.UInt8.(x *^ y)
-//     | Unsigned, W16 -> FStar.UInt16.(x *^ y)
-//     | Unsigned, W31 -> FStar.UInt31.(x *^ y)
-//     | Unsigned, W32 -> FStar.UInt32.(x *^ y)
-//     | Unsigned, W63 -> FStar.UInt63.(x *^ y)
-//     | Unsigned, W64 -> FStar.UInt64.(x *^ y)
-//     | Signed, W8 -> FStar.Int8.(x *^ y)
-//     | Signed, W16 -> FStar.Int16.(x *^ y)
-//     | Signed, W31 -> FStar.Int31.(x *^ y)
-//     | Signed, W32 -> FStar.Int32.(x *^ y)
-//     | Signed, W63 -> FStar.Int63.(x *^ y)
-//     | Signed, W64 -> FStar.Int64.(x *^ y)
-//     | Signed, W128 -> FStar.Int128.(x *^ y)
-
-// [@mark_for_norm]
-// unfold
-// private
-// let ( * ) (#s1:signedness) (#w1:width{w1 <> W128}) (#s2:signedness) (#w2:width{w2 <> W128})
-//           (x:int_t s1 w1) (y:int_t s2 w2{join_within_bounds x y (v x * v y)})
-//   : Tot   (z:norm (norm_join (join_types x y)))
-//   = x `multiplication` y
-
-// [@mark_for_norm]
-// unfold
-// let ( *? ) (#w:width{w <> W128})
-//            (x:int_t Unsigned w)
-//            (y:int_t Unsigned w)
-//   : Tot    (z:int_t Unsigned w) //{within_bounds Unsigned w (v x * v y) ==> norm (v z == v x * v y)})
-//   = match w with
-//     | Winfinite -> x * y
-//     | W8 -> FStar.UInt8.(x *?^ y)
-//     | W16 -> FStar.UInt16.(x *?^ y)
-//     | W31 -> FStar.UInt31.(x *?^ y)
-//     | W32 -> FStar.UInt32.(x *?^ y)
-//     | W63 -> FStar.UInt63.(x *?^ y)
-//     | W64 -> FStar.UInt64.(x *?^ y)
-
-// [@mark_for_norm]
-// unfold
-// let ( *% ) (#w:fixed_width{w <> W128})
-//            (x:int_t Unsigned w)
-//            (y:int_t Unsigned w)
-//   : Tot    (z:int_t Unsigned w) //{norm (v z == modulo Unsigned (v x * v y) (pow2 (nat_of_fixed_width w)))})
-//   = match w with
-//     | W8 -> FStar.UInt8.(x *%^ y)
-//     | W16 -> FStar.UInt16.(x *%^ y)
-//     | W31 -> FStar.UInt31.(x *%^ y)
-//     | W32 -> FStar.UInt32.(x *%^ y)
-//     | W63 -> FStar.UInt63.(x *%^ y)
-//     | W64 -> FStar.UInt64.(x *%^ y)
-
-// [@mark_for_norm]
-// inline_for_extraction
-// let nat        = int_t Unsigned Winfinite
-
-// [@mark_for_norm]
-// inline_for_extraction
-// let uint_8   = int_t Unsigned W8
-
-// [@mark_for_norm]
-// inline_for_extraction
-// let uint_16  = int_t Unsigned W16
-
-// [@mark_for_norm]
-// inline_for_extraction
-// let uint_31  = int_t Unsigned W31
-
-// [@mark_for_norm]
-// inline_for_extraction
-// let uint_32  = int_t Unsigned W32
-
-// [@mark_for_norm]
-// inline_for_extraction
-// let uint_63  = int_t Unsigned W63
-
-// [@mark_for_norm]
-// inline_for_extraction
-// let uint_64  = int_t Unsigned W64
-
-// [@mark_for_norm]
-// inline_for_extraction
-// let int       = int_t Signed Winfinite
-
-// [@mark_for_norm]
-// inline_for_extraction
-// let int_8   = int_t Signed W8
-
-// [@mark_for_norm]
-// inline_for_extraction
-// let int_16  = int_t Signed W16
-
-// [@mark_for_norm]
-// inline_for_extraction
-// let int_31  = int_t Signed W31
-
-// [@mark_for_norm]
-// inline_for_extraction
-// let int_32  = int_t Signed W32
-
-// [@mark_for_norm]
-// inline_for_extraction
-// let int_63  = int_t Signed W63
-
-// [@mark_for_norm]
-// inline_for_extraction
-// let int_64  = int_t Signed W64
-
-// [@mark_for_norm]
-// inline_for_extraction
-// let int_128 = int_t Signed W128
-
-// [@mark_for_norm]
-// unfold
-// let ok (#s1:signedness) (#w1:width)
-//        (#s2:signedness) (#w2:width)
-//        (op:(int_t Signed Winfinite
-//           -> int_t Signed Winfinite
-//           -> int_t Signed Winfinite))
-//        (x:int_t s1 w1)
-//        (y:int_t s2 w2)
-//    = join_within_bounds x y (op (v x) (v y))
-
-// ////////////////////////////////////////////////////////////////////////////////
-// //Test
-// ////////////////////////////////////////////////////////////////////////////////
-// let f_int (x:int) (y:int) = x + y
-// let f_nat (x:nat) (y:nat) = x + y
-// let f_uint_8 (x:uint_8) (y:uint_8{ok (+) x y}) = x + y
-// let f_int_16 (x:int_16) (y:int_16{ok (+) x y}) = x + y
-// let g (x:uint_32) (y:uint_32{// ok (+) y y /\
-//   ok (+) x (y + y) }) = () //x + (y + y)
-// let h (x:Prims.nat) (y:Prims.nat): nat  = u x + u y
-// (* TODO: A bit boring ... *)
-// (* let op_Slash_Hat = div *)
-// (* let op_Percent_Hat = rem *)
-// (* let op_Hat_Hat = logxor *)
-// (* let op_Amp_Hat = logand *)
-// (* let op_Bar_Hat = logor *)
-// (* let op_Less_Less_Hat = shift_left *)
-// (* let op_Greater_Greater_Hat = shift_right *)
-// (* let op_Equals_Hat = eq *)
-// (* let op_Greater_Hat = gt *)
-// (* let op_Greater_Equals_Hat = gte *)
-// (* let op_Less_Hat = lt *)
-// (* let op_Less_Equals_Hat = lte *)
+unfold
+let ok (#s:signedness) (#w:width)
+       (op:(int_t Signed Winfinite
+          -> int_t Signed Winfinite
+          -> int_t Signed Winfinite))
+       (x:int_t s w)
+       (y:int_t s w)
+   = normalize (within_bounds s w (op (v x) (v y)))
+////////////////////////////////////////////////////////////////////////////////
+//Test
+////////////////////////////////////////////////////////////////////////////////
+let f_int (x:int) (y:int) = x + y
+let f_nat (x:nat) (y:nat) = x + y
+let f_uint_8 (x:uint_8) (y:uint_8{ok (+) x y}) = x + y
+let f_int_16 (x:int_16) (y:int_16{ok (+) x y}) = x + y
+let g (x:uint_32) (y:uint_32{ok ( * ) y y /\ ok (+) x (y * y)}) = x + y * y
+let h (x:Prims.nat) (y:Prims.nat): nat  = u x + u y
+(* TODO: A bit boring ... *)
+(* let op_Slash_Hat = div *)
+(* let op_Percent_Hat = rem *)
+(* let op_Hat_Hat = logxor *)
+(* let op_Amp_Hat = logand *)
+(* let op_Bar_Hat = logor *)
+(* let op_Less_Less_Hat = shift_left *)
+(* let op_Greater_Greater_Hat = shift_right *)
+(* let op_Equals_Hat = eq *)
+(* let op_Greater_Hat = gt *)
+(* let op_Greater_Equals_Hat = gte *)
+(* let op_Less_Hat = lt *)
+(* let op_Less_Equals_Hat = lte *)
